\begin{theorem}
\label{thm:inference-sound-strong}
  \emph{Forall} i,s,$R$,$I$,$c$,$\F$, if $\stable(\R,I)$ and $c \elabsto \F$,
  then:\\\vspace*{-0.2cm}
  \begin{smathpar}
  \begin{array}{c}
  \R \vdash \hoare{\lambda(\stl,\stg).~\stl=s \conj
  I(\stg)}{c}{\lambda(\stl,\stg).\stl = s \cup \F(s,\stg)}
  \end{array}
  \end{smathpar}
\end{theorem}
\begin{proof}
Hypothesis:
\begin{smathpar}
\begin{array}{lr}
  \stable(\R,I) & H1\\
  c \elabsto \F & H2\\
\end{array}
\end{smathpar}
Proof by induction on $H2$. The cases for SQL statements follow from
the corresponding RG rules trivially. \C{LET}, \C{IF-THEN-ELSE}, and
sequence case proof follows from the inductive hypothesis. The only
interesting case is \C{FOREACH}, where the corresponding RG rule
requires a loop invariant ($\psi$). The loop invariant is as
following: $\psi(\stl,\stg) \Leftrightarrow \stl = y\bind(\lambda
z.~\F_c(\stl,\stg)$, where $\F_c$ is the transformer of the loop body.
% \begin{itemize}
%   \item \C{INSERT}: $\F$ is:
%   \begin{smathpar}
%   \begin{array}{c}
%     \stabilize{\lambda(\stl,\stg).~
%     \{ y \,|\, y = \{x \with r.\delf=\mathit{false};\, \txnf = i\} \}}
%   \end{array}
%   \end{smathpar}
%   If $\F$ is stable, we need to show the following:
%   \begin{smathpar}
%   \begin{array}{c}
%     \R \vdash \hoare{\lambda(\stl,\stg).~\stl=\emptyset \conj
%       I(\stg)}{\inserte{x}} {\lambda(\stl,\stg).\stl \subseteq \{ y
%       \,|\, y = \{x \with r.\delf=\mathit{false};\, \txnf = i\}}
%   \end{array}
%   \end{smathpar}
%   Which directly follows from the the RG rule for Insert. Since
%   $\C{INSERT}$ doesn't read $\stg$, the proof is the same even when
%   $\F$ is unstable.

%   \item \C{UPDATE}: $\F$ is:
%   \begin{smathpar}
%   \begin{array}{c}
%     \stabilize{\lambda(\stl,\stg).~ \stg \bind G }
%   \end{array}
%   \end{smathpar}
%   Where $G$ is $\lambda y.~ \itel{[y/x]e_2}
%   {\{[y/x]e_1 \with \idf=r.\idf;\,\delf = y.\delf;\,\txnf=i \}}
%   {\emptyset}$.
%   When 
% \end{itemize}
\end{proof}

\begin{theorem}
\label{thm:inference-sound}
  \emph{Forall} i,$R$,$I$,$c$,$\F$, if $\stable(\R,I)$ and $c \elabsto \F$,
  then:\\\vspace*{-0.2cm}
  \begin{smathpar}
  \begin{array}{c}
  \R \vdash \hoare{\lambda(\stl,\stg).~\stl=\emptyset \conj
  I(\stg)}{c}{\lambda(\stl,\stg).\stl = \F(\emptyset,\stg)}
  \end{array}
  \end{smathpar}
\end{theorem}
\begin{proof}
  Follows from the stronger version of this theorem
  (Theorem~\ref{thm:inference-sound-strong}) by substituting
  $\emptyset$ for $s$.
\end{proof}
